examples/pseudo_bool/cp_encoding/cp_to_ilp_logicalScript.sml
@@ -227,25 +227,6 @@ Proof
   simp[cencode_or_aux_def,encode_or_aux_def,enc_rel_List_refl_mul]
 QED
 
-(* encodes that the values of the Boolean variables X and Y are equal *)
-Definition encode_bvar_eq_def:
-  encode_bvar_eq X Y =
-  [
-    ([], [(1, Pos X);(-1, Pos Y)], 0);
-    ([], [(1, Pos Y);(-1, Pos X)], 0)
-  ]
-End
-
-Theorem encode_bvar_eq_sem[simp]:
-  EVERY (λx. iconstraint_sem x (wi,wb)) (encode_bvar_eq X Y) ⇔
-  wb X = wb Y
-Proof
-  simp[encode_bvar_eq_def,iconstraint_sem_def]>>
-  Cases_on‘wb X’>>
-  Cases_on‘wb Y’>>
-  fs[]
-QED
-
 (* encodes that the values of the Boolean variables X, Y and Z satisfy:
    X xor Y = Z
 *)
